<?xml version="1.0"?>
<rdf:RDF xmlns="http://rescue-mate.de/ontology/wikidata-bridge/"
     xml:base="http://rescue-mate.de/ontology/wikidata-bridge/"
     xmlns:dc="http://purl.org/dc/elements/1.1/"
     xmlns:obo="http://purl.obolibrary.org/obo/"
     xmlns:owl="http://www.w3.org/2002/07/owl#"
     xmlns:rdf="http://www.w3.org/1999/02/22-rdf-syntax-ns#"
     xmlns:xml="http://www.w3.org/XML/1998/namespace"
     xmlns:xsd="http://www.w3.org/2001/XMLSchema#"
     xmlns:foaf="http://xmlns.com/foaf/0.1/"
     xmlns:rdfs="http://www.w3.org/2000/01/rdf-schema#"
     xmlns:terms="http://purl.org/dc/terms/">
    <owl:Ontology rdf:about="http://rescue-mate.de/ontology/wikidata-bridge">
        <owl:versionIRI rdf:resource="http://rescue-mate.de/ontology/wikidata-bridge/0.1.0"/>
        <owl:imports rdf:resource="http://purl.obolibrary.org/obo/bfo/2019-08-26/bfo.owl"/>
    </owl:Ontology>
    


    <!-- 
    ///////////////////////////////////////////////////////////////////////////////////////
    //
    // Classes
    //
    ///////////////////////////////////////////////////////////////////////////////////////
     -->

    


    <!-- https://www.wikidata.org/wiki/Q105731 -->

    <owl:Class rdf:about="https://www.wikidata.org/wiki/Q105731">
        <rdfs:subClassOf rdf:resource="https://www.wikidata.org/wiki/Q333170"/>
        <rdfs:comment xml:lang="de">Abstiegsbauwerk mit einer festen Kammer und wechselndem Wasserstand</rdfs:comment>
        <rdfs:comment xml:lang="en">fall structure with a fixed chamber in which the water level changes</rdfs:comment>
        <rdfs:comment xml:lang="fr">ouvrage d&apos;art hydraulique implanté dans un canal, un cours ou une étendue d&apos;eau pour maîtriser sa profondeur ou son débit</rdfs:comment>
        <rdfs:label xml:lang="de">Schiffsschleuse</rdfs:label>
        <rdfs:label xml:lang="en">lock</rdfs:label>
        <rdfs:label xml:lang="fr">écluse</rdfs:label>
    </owl:Class>
    


    <!-- https://www.wikidata.org/wiki/Q106559804 -->

    <owl:Class rdf:about="https://www.wikidata.org/wiki/Q106559804">
        <rdfs:subClassOf rdf:resource="https://www.wikidata.org/wiki/Q24229398"/>
        <rdfs:comment xml:lang="de">Art von Vermittler</rdfs:comment>
        <rdfs:comment xml:lang="en">class of agents</rdfs:comment>
        <rdfs:comment xml:lang="fr">type d&apos;agent</rdfs:comment>
        <rdfs:label xml:lang="de">Person oder Organisation</rdfs:label>
        <rdfs:label xml:lang="en">person or organization</rdfs:label>
        <rdfs:label xml:lang="fr">personne ou organisation</rdfs:label>
    </owl:Class>
    


    <!-- https://www.wikidata.org/wiki/Q106668099 -->

    <owl:Class rdf:about="https://www.wikidata.org/wiki/Q106668099">
        <rdfs:subClassOf rdf:resource="https://www.wikidata.org/wiki/Q131085629"/>
        <rdfs:subClassOf rdf:resource="https://www.wikidata.org/wiki/Q488383"/>
        <rdfs:comment xml:lang="fr">en bibliothéconomie, agent collectif composé de personnes organisées dans un but ou une activité commune; l&apos;agent collectif comprend les personnes morales et les familles</rdfs:comment>
        <rdfs:comment xml:lang="de">in der Bibliothekswissenschaft ein Kollektivagent, der aus Personen besteht, die für einen gemeinsamen Zweck oder eine gemeinsame Tätigkeit organisiert sind; Kollektivagent umfasst Körperschaften und Familien</rdfs:comment>
        <rdfs:comment xml:lang="en">in library science, a collective agent that is composed of persons who are organized for a common purpose or activity; collective agent includes corporate bodies and families</rdfs:comment>
        <rdfs:label xml:lang="de">Körperschaft</rdfs:label>
        <rdfs:label xml:lang="fr">collectivité</rdfs:label>
        <rdfs:label xml:lang="en">corporate body</rdfs:label>
    </owl:Class>
    


    <!-- https://www.wikidata.org/wiki/Q107589046 -->

    <owl:Class rdf:about="https://www.wikidata.org/wiki/Q107589046">
        <rdfs:subClassOf rdf:resource="https://www.wikidata.org/wiki/Q2466889"/>
        <rdfs:comment xml:lang="en">hydraulic structure between two waterways with a different water level, which serves to transport water or ships between the waterways</rdfs:comment>
        <rdfs:comment xml:lang="de">hydraulisches Bauwerk zwischen zwei Wasserkörpern mit unterschiedlichem Pegel, das dazu dient, Wasser oder Wasserfahrzeuge auf ein anderes Niveau zu bringen</rdfs:comment>
        <rdfs:label xml:lang="en">sluice</rdfs:label>
    </owl:Class>
    


    <!-- https://www.wikidata.org/wiki/Q123349660 -->

    <owl:Class rdf:about="https://www.wikidata.org/wiki/Q123349660">
        <rdfs:subClassOf rdf:resource="http://purl.obolibrary.org/obo/BFO_0000040"/>
        <rdfs:comment xml:lang="de">Geoobjekt</rdfs:comment>
        <rdfs:comment xml:lang="en">entity that may be assigned mostly stable geographic coordinates and/or geocoded</rdfs:comment>
        <rdfs:comment xml:lang="fr">entité qui peut avoir des coordonnées géographiques et/ou être géocodé</rdfs:comment>
        <rdfs:label xml:lang="fr">entité cartographiable</rdfs:label>
        <rdfs:label xml:lang="en">geolocatable entity</rdfs:label>
        <rdfs:label xml:lang="de">geolokalisierbares Objekt</rdfs:label>
    </owl:Class>
    


    <!-- https://www.wikidata.org/wiki/Q12569864 -->

    <owl:Class rdf:about="https://www.wikidata.org/wiki/Q12569864">
        <rdfs:subClassOf rdf:resource="https://www.wikidata.org/wiki/Q106559804"/>
        <rdfs:comment xml:lang="en">one of the assumptions made in generally accepted accounting principles</rdfs:comment>
        <rdfs:label xml:lang="en">economic entity</rdfs:label>
        <rdfs:label xml:lang="fr">entité économique</rdfs:label>
    </owl:Class>
    


    <!-- https://www.wikidata.org/wiki/Q131085629 -->

    <owl:Class rdf:about="https://www.wikidata.org/wiki/Q131085629">
        <rdfs:subClassOf rdf:resource="https://www.wikidata.org/wiki/Q24229398"/>
        <rdfs:comment xml:lang="fr">agent qui est un groupement ou une association de deux ou plusieurs personnes portant un nom particulier et disposant de la faculté d’agir collectivement</rdfs:comment>
        <rdfs:comment xml:lang="en">an agent who is a gathering or organization of two or more persons that bears a particular name and that is capable of acting as a unit</rdfs:comment>
        <rdfs:comment xml:lang="de">ein Akteur, bei dem es sich um eine Zusammenkunft oder eine Organisation von zwei oder mehreren Personen handelt, die der einen bestimmten Namen trägt und imstande ist, als Einheit zu handeln</rdfs:comment>
        <rdfs:label xml:lang="de">Gemeinschaftlicher Akteur</rdfs:label>
        <rdfs:label xml:lang="fr">agent collectif</rdfs:label>
        <rdfs:label xml:lang="en">collective agent</rdfs:label>
    </owl:Class>
    


    <!-- https://www.wikidata.org/wiki/Q1411945 -->

    <owl:Class rdf:about="https://www.wikidata.org/wiki/Q1411945">
        <rdfs:subClassOf rdf:resource="https://www.wikidata.org/wiki/Q811979"/>
        <rdfs:comment xml:lang="de">Bauwerk mit komplexer Baustatik</rdfs:comment>
        <rdfs:comment xml:lang="fr">construction civile</rdfs:comment>
        <rdfs:comment xml:lang="en">type of construction</rdfs:comment>
        <rdfs:label xml:lang="de">Ingenieurbauwerk</rdfs:label>
        <rdfs:label xml:lang="en">civil engineering construction</rdfs:label>
        <rdfs:label xml:lang="fr">ouvrage d&apos;art</rdfs:label>
    </owl:Class>
    


    <!-- https://www.wikidata.org/wiki/Q14524070 -->

    <owl:Class rdf:about="https://www.wikidata.org/wiki/Q14524070">
        <rdfs:subClassOf rdf:resource="https://www.wikidata.org/wiki/Q1411945"/>
        <rdfs:comment xml:lang="de">Hebevorrichtung für Wasser</rdfs:comment>
        <rdfs:comment xml:lang="en">acility which is part of a water supply network and is used to transport water up an incline</rdfs:comment>
        <rdfs:label xml:lang="de">Schöpfwerk</rdfs:label>
        <rdfs:label xml:lang="fr">station de pompage des eaux</rdfs:label>
        <rdfs:label xml:lang="en">water pumping station</rdfs:label>
    </owl:Class>
    


    <!-- https://www.wikidata.org/wiki/Q15848142 -->

    <owl:Class rdf:about="https://www.wikidata.org/wiki/Q15848142">
        <rdfs:subClassOf rdf:resource="https://www.wikidata.org/wiki/Q2466889"/>
        <rdfs:comment xml:lang="de">Bauwerk, um Binnenland vor Hochwasser zu schützen</rdfs:comment>
        <rdfs:comment xml:lang="en">hydraulic structure used to prevent tidal flooding</rdfs:comment>
        <rdfs:label xml:lang="de">Sperrwerk</rdfs:label>
        <rdfs:label xml:lang="en">Tidal barrier</rdfs:label>
        <rdfs:label xml:lang="fr">barrière contre les inondations</rdfs:label>
    </owl:Class>
    


    <!-- https://www.wikidata.org/wiki/Q223557 -->

    <owl:Class rdf:about="https://www.wikidata.org/wiki/Q223557">
        <rdfs:subClassOf rdf:resource="http://purl.obolibrary.org/obo/BFO_0000040"/>
        <rdfs:comment xml:lang="de">Ansammlung von Masse, die eine Einheit bildet</rdfs:comment>
        <rdfs:comment xml:lang="en">singular aggregation of substance(s) such as matter or radiation, with overall properties such as mass, position or momentum</rdfs:comment>
        <rdfs:label xml:lang="de">Körper</rdfs:label>
        <rdfs:label xml:lang="fr">objet physique</rdfs:label>
        <rdfs:label xml:lang="en">physical object</rdfs:label>
    </owl:Class>
    


    <!-- https://www.wikidata.org/wiki/Q2345125 -->

    <owl:Class rdf:about="https://www.wikidata.org/wiki/Q2345125">
        <rdfs:subClassOf rdf:resource="https://www.wikidata.org/wiki/Q105731"/>
        <rdfs:comment xml:lang="en">adjustable gate used to control water flow</rdfs:comment>
        <rdfs:comment xml:lang="de">bewegliches Schott zum Absperren eines niederen Wasserstandes</rdfs:comment>
        <rdfs:label xml:lang="de">Fluttor</rdfs:label>
        <rdfs:label xml:lang="en">floodgate</rdfs:label>
        <rdfs:label xml:lang="fr">vanne contre les inondations</rdfs:label>
    </owl:Class>
    


    <!-- https://www.wikidata.org/wiki/Q24229398 -->

    <owl:Class rdf:about="https://www.wikidata.org/wiki/Q24229398">
        <rdfs:subClassOf rdf:resource="http://purl.obolibrary.org/obo/BFO_0000004"/>
        <rdfs:comment xml:lang="de">Entität, die Aktionen ausführen kann</rdfs:comment>
        <rdfs:comment xml:lang="en">distinct and identifiable entity capable of performing actions</rdfs:comment>
        <rdfs:comment xml:lang="fr">entité individuelle et identifiable qui peut conduire des actions (comme une personne physique ou une organisation)</rdfs:comment>
        <rdfs:label xml:lang="de">Akteur</rdfs:label>
        <rdfs:label xml:lang="en">agent</rdfs:label>
        <rdfs:label xml:lang="fr">agent</rdfs:label>
    </owl:Class>
    


    <!-- https://www.wikidata.org/wiki/Q2466889 -->

    <owl:Class rdf:about="https://www.wikidata.org/wiki/Q2466889">
        <rdfs:subClassOf rdf:resource="https://www.wikidata.org/wiki/Q1411945"/>
        <rdfs:subClassOf rdf:resource="https://www.wikidata.org/wiki/Q811979"/>
        <rdfs:comment xml:lang="de">Bauwerk, das einen natürlichen Wasserlauf verändert</rdfs:comment>
        <rdfs:comment xml:lang="en">artificial structure which disrupts the natural flow of water</rdfs:comment>
        <rdfs:comment xml:lang="fr">type d&apos;ouvrage d&apos;art</rdfs:comment>
        <rdfs:label xml:lang="en">hydraulic structure</rdfs:label>
        <rdfs:label xml:lang="de">hydraulisches Bauwerk</rdfs:label>
        <rdfs:label xml:lang="fr">ouvrage hydraulique</rdfs:label>
    </owl:Class>
    


    <!-- https://www.wikidata.org/wiki/Q27096213 -->

    <owl:Class rdf:about="https://www.wikidata.org/wiki/Q27096213">
        <rdfs:subClassOf rdf:resource="https://www.wikidata.org/wiki/Q123349660"/>
        <rdfs:comment xml:lang="de">Ort oder Objekt</rdfs:comment>
        <rdfs:comment xml:lang="fr">lieu ou entité susceptible de l&apos;être</rdfs:comment>
        <rdfs:comment xml:lang="en">relatively stationary place or entity that can be geographically identified, located, or described</rdfs:comment>
        <rdfs:label xml:lang="fr">entité géographique</rdfs:label>
        <rdfs:label xml:lang="de">geografische Entität</rdfs:label>
        <rdfs:label xml:lang="en">geographic entity</rdfs:label>
    </owl:Class>
    


    <!-- https://www.wikidata.org/wiki/Q333170 -->

    <owl:Class rdf:about="https://www.wikidata.org/wiki/Q333170">
        <rdfs:subClassOf rdf:resource="https://www.wikidata.org/wiki/Q107589046"/>
        <rdfs:comment xml:lang="de">Verkehrswasserbauwerk, das Wasserfahrzeugen das Überwinden eines Höhenunterschiedes ermöglicht</rdfs:comment>
        <rdfs:comment xml:lang="en">structure that allows vessels to overcome a fall in a waterway</rdfs:comment>
        <rdfs:label xml:lang="de">Abstiegsbauwerk</rdfs:label>
        <rdfs:label xml:lang="en">fall structure</rdfs:label>
    </owl:Class>
    


    <!-- https://www.wikidata.org/wiki/Q446013 -->

    <owl:Class rdf:about="https://www.wikidata.org/wiki/Q446013">
        <rdfs:subClassOf rdf:resource="https://www.wikidata.org/wiki/Q2466889"/>
        <rdfs:comment xml:lang="de">Anlage, mit der Wasser aus einem niedriger gelegenen Gewässer in ein höher gelegenes gepumpt wird</rdfs:comment>
        <rdfs:comment xml:lang="en">facilities including pumps and equipment for pumping fluids from one place to another</rdfs:comment>
        <rdfs:label xml:lang="de">Pumpwerk</rdfs:label>
        <rdfs:label xml:lang="en">pumping station</rdfs:label>
        <rdfs:label xml:lang="fr">station de pompage</rdfs:label>
    </owl:Class>
    


    <!-- https://www.wikidata.org/wiki/Q510255 -->

    <owl:Class rdf:about="https://www.wikidata.org/wiki/Q510255">
        <rdfs:subClassOf rdf:resource="https://www.wikidata.org/wiki/Q107589046"/>
        <rdfs:comment xml:lang="fr">ouvrage de vidange de digue</rdfs:comment>
        <rdfs:comment xml:lang="de">verschließbarer Gewässerdurchlass in einem Deich</rdfs:comment>
        <rdfs:label xml:lang="de">Siel</rdfs:label>
        <rdfs:label xml:lang="en">discharge sluice</rdfs:label>
        <rdfs:label xml:lang="fr">écluse de chasse</rdfs:label>
    </owl:Class>
    


    <!-- https://www.wikidata.org/wiki/Q618123 -->

    <owl:Class rdf:about="https://www.wikidata.org/wiki/Q618123">
        <rdfs:subClassOf rdf:resource="https://www.wikidata.org/wiki/Q27096213"/>
        <rdfs:comment xml:lang="de">Objekt, welches mittels Geodaten eindeutig referenzierbar war bzw. ist</rdfs:comment>
        <rdfs:comment xml:lang="en">components of planets that can be geographically located</rdfs:comment>
        <rdfs:comment xml:lang="fr">entité identifiée de manière unique par une donnée spatiale</rdfs:comment>
        <rdfs:label xml:lang="en">geographical feature</rdfs:label>
        <rdfs:label xml:lang="de">geographisches Objekt</rdfs:label>
        <rdfs:label xml:lang="fr">objet géographique</rdfs:label>
    </owl:Class>
    


    <!-- https://www.wikidata.org/wiki/Q811430 -->

    <owl:Class rdf:about="https://www.wikidata.org/wiki/Q811430">
        <rdfs:subClassOf rdf:resource="https://www.wikidata.org/wiki/Q618123"/>
        <rdfs:comment xml:lang="de">Konstruktion von Bauwerken und Gebäuden</rdfs:comment>
        <rdfs:comment xml:lang="en">artificially constructed entity meant to remain at a fixed geographic location</rdfs:comment>
        <rdfs:comment xml:lang="fr">objet physique</rdfs:comment>
        <rdfs:label xml:lang="de">Baukonstruktion</rdfs:label>
        <rdfs:label xml:lang="en">fixed construction</rdfs:label>
        <rdfs:label xml:lang="fr">structure construite</rdfs:label>
    </owl:Class>
    


    <!-- https://www.wikidata.org/wiki/Q811979 -->

    <owl:Class rdf:about="https://www.wikidata.org/wiki/Q811979">
        <rdfs:subClassOf rdf:resource="https://www.wikidata.org/wiki/Q811430"/>
        <rdfs:comment xml:lang="de">Konstruktion mit ruhendem Kontakt zum Untergrund, z. B. Straße, Brücke, Fundament</rdfs:comment>
        <rdfs:comment xml:lang="fr">construction dont la conception a été pensée</rdfs:comment>
        <rdfs:comment xml:lang="en">human-designed and -made structure</rdfs:comment>
        <rdfs:label xml:lang="de">Bauwerk</rdfs:label>
        <rdfs:label xml:lang="en">architectural structure</rdfs:label>
        <rdfs:label xml:lang="fr">structure architecturale</rdfs:label>
    </owl:Class>
    


    <!-- https://www.wikidata.org/wiki/Q99527517 -->

    <owl:Class rdf:about="https://www.wikidata.org/wiki/Q99527517">
        <rdfs:subClassOf rdf:resource="http://purl.obolibrary.org/obo/BFO_0000001"/>
        <rdfs:comment xml:lang="en">entity that is a composite of other entities</rdfs:comment>
        <rdfs:comment xml:lang="fr">entité qui est un composite d&apos;autres entités</rdfs:comment>
        <rdfs:label xml:lang="en">collective entity</rdfs:label>
        <rdfs:label xml:lang="fr">entité composée</rdfs:label>
    </owl:Class>
</rdf:RDF>



<!-- Generated by the OWL API (version 4.5.29.2024-05-13T12:11:03Z) https://github.com/owlcs/owlapi -->

