<?xml version="1.0"?>
<rdf:RDF xmlns="http://rescue-mate.de/ontology/wikidata-bridge/"
     xml:base="http://rescue-mate.de/ontology/wikidata-bridge/"
     xmlns:dc="http://purl.org/dc/elements/1.1/"
     xmlns:obo="http://purl.obolibrary.org/obo/"
     xmlns:owl="http://www.w3.org/2002/07/owl#"
     xmlns:rdf="http://www.w3.org/1999/02/22-rdf-syntax-ns#"
     xmlns:xml="http://www.w3.org/XML/1998/namespace"
     xmlns:xsd="http://www.w3.org/2001/XMLSchema#"
     xmlns:foaf="http://xmlns.com/foaf/0.1/"
     xmlns:rdfs="http://www.w3.org/2000/01/rdf-schema#"
     xmlns:terms="http://purl.org/dc/terms/">
    <owl:Ontology rdf:about="http://rescue-mate.de/ontology/wikidata-bridge">
        <owl:versionIRI rdf:resource="http://rescue-mate.de/ontology/wikidata-bridge/0.3.0"/>
        <owl:imports rdf:resource="http://purl.obolibrary.org/obo/bfo/2019-08-26/bfo.owl"/>
    </owl:Ontology>
    


    <!-- 
    ///////////////////////////////////////////////////////////////////////////////////////
    //
    // Classes
    //
    ///////////////////////////////////////////////////////////////////////////////////////
     -->

    


    <!-- https://www.wikidata.org/wiki/Q10273457 -->

    <owl:Class rdf:about="https://www.wikidata.org/wiki/Q10273457">
        <rdfs:subClassOf rdf:resource="https://www.wikidata.org/wiki/Q223557"/>
        <rdfs:comment xml:lang="de">allgemeiner Sammelbegriff für alle Gegenstände, die benötigt werden um eine bestimmte Tätigkeit auszuüben</rdfs:comment>
        <rdfs:comment xml:lang="en">collective term for all physical items that are required to exercise a certain activity</rdfs:comment>
        <rdfs:comment xml:lang="fr">terme générique pour tous les objets qui sont nécessaires pour exercer une activité</rdfs:comment>
        <rdfs:label xml:lang="de">Ausrüstung</rdfs:label>
        <rdfs:label xml:lang="en">equipment</rdfs:label>
        <rdfs:label xml:lang="fr">équipement</rdfs:label>
    </owl:Class>
    


    <!-- https://www.wikidata.org/wiki/Q105731 -->

    <owl:Class rdf:about="https://www.wikidata.org/wiki/Q105731">
        <rdfs:subClassOf rdf:resource="https://www.wikidata.org/wiki/Q333170"/>
        <rdfs:comment xml:lang="de">Abstiegsbauwerk mit einer festen Kammer und wechselndem Wasserstand</rdfs:comment>
        <rdfs:comment xml:lang="en">fall structure with a fixed chamber in which the water level changes</rdfs:comment>
        <rdfs:comment xml:lang="fr">ouvrage d&apos;art hydraulique implanté dans un canal, un cours ou une étendue d&apos;eau pour maîtriser sa profondeur ou son débit</rdfs:comment>
        <rdfs:label xml:lang="de">Schiffsschleuse</rdfs:label>
        <rdfs:label xml:lang="en">lock</rdfs:label>
        <rdfs:label xml:lang="fr">écluse</rdfs:label>
    </owl:Class>
    


    <!-- https://www.wikidata.org/wiki/Q106559804 -->

    <owl:Class rdf:about="https://www.wikidata.org/wiki/Q106559804">
        <rdfs:subClassOf rdf:resource="https://www.wikidata.org/wiki/Q24229398"/>
        <rdfs:comment xml:lang="de">Art von Vermittler</rdfs:comment>
        <rdfs:comment xml:lang="en">class of agents</rdfs:comment>
        <rdfs:comment xml:lang="fr">type d&apos;agent</rdfs:comment>
        <rdfs:label xml:lang="de">Person oder Organisation</rdfs:label>
        <rdfs:label xml:lang="en">person or organization</rdfs:label>
        <rdfs:label xml:lang="fr">personne ou organisation</rdfs:label>
    </owl:Class>
    


    <!-- https://www.wikidata.org/wiki/Q106668099 -->

    <owl:Class rdf:about="https://www.wikidata.org/wiki/Q106668099">
        <rdfs:subClassOf rdf:resource="http://purl.obolibrary.org/obo/BFO_0000030"/>
        <rdfs:subClassOf rdf:resource="https://www.wikidata.org/wiki/Q131085629"/>
        <rdfs:comment xml:lang="fr">en bibliothéconomie, agent collectif composé de personnes organisées dans un but ou une activité commune; l&apos;agent collectif comprend les personnes morales et les familles</rdfs:comment>
        <rdfs:comment xml:lang="de">in der Bibliothekswissenschaft ein Kollektivagent, der aus Personen besteht, die für einen gemeinsamen Zweck oder eine gemeinsame Tätigkeit organisiert sind; Kollektivagent umfasst Körperschaften und Familien</rdfs:comment>
        <rdfs:comment xml:lang="en">in library science, a collective agent that is composed of persons who are organized for a common purpose or activity; collective agent includes corporate bodies and families</rdfs:comment>
        <rdfs:label xml:lang="de">Körperschaft</rdfs:label>
        <rdfs:label xml:lang="fr">collectivité</rdfs:label>
        <rdfs:label xml:lang="en">corporate body</rdfs:label>
    </owl:Class>
    


    <!-- https://www.wikidata.org/wiki/Q106839123 -->

    <owl:Class rdf:about="https://www.wikidata.org/wiki/Q106839123">
        <rdfs:subClassOf rdf:resource="https://www.wikidata.org/wiki/Q10273457"/>
        <rdfs:comment xml:lang="de">Einrichtungen oder Nutztiere, die der Beförderung von Personen und Gütern dienen</rdfs:comment>
        <rdfs:comment xml:lang="en">any form of vehicle or system used to transport people or goods from one place to another</rdfs:comment>
        <rdfs:comment xml:lang="fr">véhicule ou équipement utilisé pour le transport de personnes ou de marchandises</rdfs:comment>
        <rdfs:label xml:lang="de">Verkehrsmittel</rdfs:label>
        <rdfs:label xml:lang="en">means of transport</rdfs:label>
        <rdfs:label xml:lang="fr">moyen de transport</rdfs:label>
    </owl:Class>
    


    <!-- https://www.wikidata.org/wiki/Q107280686 -->

    <owl:Class rdf:about="https://www.wikidata.org/wiki/Q107280686">
        <rdfs:subClassOf rdf:resource="https://www.wikidata.org/wiki/Q451967"/>
        <rdfs:comment xml:lang="en">human activity involving assistance to others and improvement of conditions for humanity</rdfs:comment>
        <rdfs:label xml:lang="fr">activité humanitaire</rdfs:label>
        <rdfs:label xml:lang="en">humanitarian activity</rdfs:label>
    </owl:Class>
    


    <!-- https://www.wikidata.org/wiki/Q107589046 -->

    <owl:Class rdf:about="https://www.wikidata.org/wiki/Q107589046">
        <rdfs:subClassOf rdf:resource="https://www.wikidata.org/wiki/Q2466889"/>
        <rdfs:comment xml:lang="en">hydraulic structure between two waterways with a different water level, which serves to transport water or ships between the waterways</rdfs:comment>
        <rdfs:comment xml:lang="de">hydraulisches Bauwerk zwischen zwei Wasserkörpern mit unterschiedlichem Pegel, das dazu dient, Wasser oder Wasserfahrzeuge auf ein anderes Niveau zu bringen</rdfs:comment>
        <rdfs:label xml:lang="en">sluice</rdfs:label>
    </owl:Class>
    


    <!-- https://www.wikidata.org/wiki/Q11019 -->

    <owl:Class rdf:about="https://www.wikidata.org/wiki/Q11019">
        <rdfs:subClassOf rdf:resource="https://www.wikidata.org/wiki/Q1183543"/>
        <rdfs:comment xml:lang="de">mechanisches Gerät mit Antriebssystem</rdfs:comment>
        <rdfs:comment xml:lang="fr">outil capable d&apos;effectuer des tâches en consommant de l&apos;énergie</rdfs:comment>
        <rdfs:comment xml:lang="en">tool containing one or more parts that uses energy to perform an intended action</rdfs:comment>
        <rdfs:label xml:lang="de">Maschine</rdfs:label>
        <rdfs:label xml:lang="en">machine</rdfs:label>
        <rdfs:label xml:lang="fr">machine</rdfs:label>
    </owl:Class>
    


    <!-- https://www.wikidata.org/wiki/Q11436 -->

    <owl:Class rdf:about="https://www.wikidata.org/wiki/Q11436">
        <rdfs:subClassOf rdf:resource="https://www.wikidata.org/wiki/Q42889"/>
        <rdfs:subClassOf rdf:resource="https://www.wikidata.org/wiki/Q7194062"/>
        <rdfs:comment xml:lang="de">Transportmittel, das innerhalb der Atmosphäre abhebt und fliegt oder fährt</rdfs:comment>
        <rdfs:comment xml:lang="en">machine that is able to fly by gaining support from the air other than the reactions of the air against the earth’s surface</rdfs:comment>
        <rdfs:comment xml:lang="fr">moyen de transport capable d&apos;évoluer au sein de l&apos;atmosphère terrestre</rdfs:comment>
        <rdfs:label xml:lang="de">Luftfahrzeug</rdfs:label>
        <rdfs:label xml:lang="en">aircraft</rdfs:label>
        <rdfs:label xml:lang="fr">aéronef</rdfs:label>
    </owl:Class>
    


    <!-- https://www.wikidata.org/wiki/Q1150070 -->

    <owl:Class rdf:about="https://www.wikidata.org/wiki/Q1150070">
        <rdfs:subClassOf rdf:resource="http://purl.obolibrary.org/obo/BFO_0000003"/>
        <rdfs:comment xml:lang="de">beschreibt Prozesse, Ereignisse oder Handlungen, welche vom Status Quo abweichen</rdfs:comment>
        <rdfs:comment xml:lang="fr">décrit les processus, les événements ou actions qui s&apos;écartent du statu quo</rdfs:comment>
        <rdfs:comment xml:lang="en">process, event or action that deviates from the present state</rdfs:comment>
        <rdfs:label xml:lang="de">Veränderung</rdfs:label>
        <rdfs:label xml:lang="en">change</rdfs:label>
        <rdfs:label xml:lang="fr">changement</rdfs:label>
    </owl:Class>
    


    <!-- https://www.wikidata.org/wiki/Q116780996 -->

    <owl:Class rdf:about="https://www.wikidata.org/wiki/Q116780996">
        <rdfs:subClassOf rdf:resource="https://www.wikidata.org/wiki/Q223557"/>
        <rdfs:comment xml:lang="de">Objekt, das zum Fliegen imstande ist</rdfs:comment>
        <rdfs:comment xml:lang="en">object capable of flight</rdfs:comment>
        <rdfs:comment xml:lang="fr">objet ayant la capacité de voler</rdfs:comment>
        <rdfs:label xml:lang="de">Flugobjekt</rdfs:label>
        <rdfs:label xml:lang="en">flying object</rdfs:label>
        <rdfs:label xml:lang="fr">objet volant</rdfs:label>
    </owl:Class>
    


    <!-- https://www.wikidata.org/wiki/Q117134054 -->

    <owl:Class rdf:about="https://www.wikidata.org/wiki/Q117134054">
        <rdfs:subClassOf rdf:resource="https://www.wikidata.org/wiki/Q481609"/>
        <rdfs:comment xml:lang="en">broad term used to include injury and psychological trauma</rdfs:comment>
        <rdfs:label xml:lang="en">trauma</rdfs:label>
    </owl:Class>
    


    <!-- https://www.wikidata.org/wiki/Q1183543 -->

    <owl:Class rdf:about="https://www.wikidata.org/wiki/Q1183543">
        <rdfs:subClassOf rdf:resource="https://www.wikidata.org/wiki/Q39546"/>
        <rdfs:comment xml:lang="en">artificial object with which something can be worked on, manufactured or effected</rdfs:comment>
        <rdfs:comment xml:lang="de">künstlicher Gegenstand, mit dem etwas bearbeitet, hergestellt oder bewirkt werden kann</rdfs:comment>
        <rdfs:comment xml:lang="fr">objet artificiel avec lequel quelque chose peut être travaillé, fabriqué ou effectué</rdfs:comment>
        <rdfs:label xml:lang="de">Gerät</rdfs:label>
        <rdfs:label xml:lang="en">appliance</rdfs:label>
        <rdfs:label xml:lang="fr">dispositif</rdfs:label>
    </owl:Class>
    


    <!-- https://www.wikidata.org/wiki/Q11858035 -->

    <owl:Class rdf:about="https://www.wikidata.org/wiki/Q11858035">
        <rdfs:subClassOf rdf:resource="https://www.wikidata.org/wiki/Q4026292"/>
        <rdfs:comment xml:lang="en">an action to give assistance provided by emergency services, teams, or individuals</rdfs:comment>
        <rdfs:comment xml:lang="de">eine Hilfsaktion, die von Rettungsdiensten, Teams oder Einzelpersonen durchgeführt wird</rdfs:comment>
        <rdfs:label xml:lang="de">Notfallmaßnahmen</rdfs:label>
        <rdfs:label xml:lang="fr">action d&apos;urgence</rdfs:label>
        <rdfs:label xml:lang="en">emergency response</rdfs:label>
    </owl:Class>
    


    <!-- https://www.wikidata.org/wiki/Q1190554 -->

    <owl:Class rdf:about="https://www.wikidata.org/wiki/Q1190554">
        <rdfs:subClassOf rdf:resource="http://purl.obolibrary.org/obo/BFO_0000003"/>
        <rdfs:comment xml:lang="de">Auftreten eines beobachtbaren Geschehens</rdfs:comment>
        <rdfs:comment xml:lang="fr">occurrence d’un fait ou objet dans l’espace-temps; instanciation d&apos;une propriété dans un objet; ce qui peut être expérimenté ou enregistré par un observateur.</rdfs:comment>
        <rdfs:comment xml:lang="en">occurrence of a fact or object in space-time; instantiation of a property in an object</rdfs:comment>
        <rdfs:label xml:lang="de">Ereignis</rdfs:label>
        <rdfs:label xml:lang="en">occurrence</rdfs:label>
        <rdfs:label xml:lang="fr">occurrence</rdfs:label>
    </owl:Class>
    


    <!-- https://www.wikidata.org/wiki/Q1229765 -->

    <owl:Class rdf:about="https://www.wikidata.org/wiki/Q1229765">
        <rdfs:subClassOf rdf:resource="https://www.wikidata.org/wiki/Q16391167"/>
        <rdfs:comment xml:lang="en">Fahrzeuge, die zur Fortbewegung auf dem oder im Wasser bestimmt sind</rdfs:comment>
        <rdfs:comment xml:lang="en">vehicles that are intended for locomotion on or in the water</rdfs:comment>
        <rdfs:comment xml:lang="fr">véhicule destiné à la locomotion sur ou dans l&apos;eau</rdfs:comment>
        <rdfs:label xml:lang="de">Wasserfahrzeug</rdfs:label>
        <rdfs:label xml:lang="fr">embarcation</rdfs:label>
        <rdfs:label xml:lang="en">watercraft</rdfs:label>
    </owl:Class>
    


    <!-- https://www.wikidata.org/wiki/Q123349660 -->

    <owl:Class rdf:about="https://www.wikidata.org/wiki/Q123349660">
        <rdfs:subClassOf rdf:resource="http://purl.obolibrary.org/obo/BFO_0000040"/>
        <rdfs:comment xml:lang="de">Geoobjekt</rdfs:comment>
        <rdfs:comment xml:lang="en">entity that may be assigned mostly stable geographic coordinates and/or geocoded</rdfs:comment>
        <rdfs:comment xml:lang="fr">entité qui peut avoir des coordonnées géographiques et/ou être géocodé</rdfs:comment>
        <rdfs:label xml:lang="fr">entité cartographiable</rdfs:label>
        <rdfs:label xml:lang="en">geolocatable entity</rdfs:label>
        <rdfs:label xml:lang="de">geolokalisierbares Objekt</rdfs:label>
    </owl:Class>
    


    <!-- https://www.wikidata.org/wiki/Q123691918 -->

    <owl:Class rdf:about="https://www.wikidata.org/wiki/Q123691918">
        <rdfs:subClassOf rdf:resource="http://purl.obolibrary.org/obo/BFO_0000030"/>
        <rdfs:comment xml:lang="de">etwas, das zur Durchführung von etwas verwendet wird</rdfs:comment>
        <rdfs:comment xml:lang="en">something used to perform an operation</rdfs:comment>
        <rdfs:label xml:lang="de">Instrument</rdfs:label>
        <rdfs:label xml:lang="fr">outil</rdfs:label>
        <rdfs:label xml:lang="en">tool</rdfs:label>
    </owl:Class>
    


    <!-- https://www.wikidata.org/wiki/Q12569864 -->

    <owl:Class rdf:about="https://www.wikidata.org/wiki/Q12569864">
        <rdfs:subClassOf rdf:resource="https://www.wikidata.org/wiki/Q106559804"/>
        <rdfs:comment xml:lang="en">one of the assumptions made in generally accepted accounting principles</rdfs:comment>
        <rdfs:label xml:lang="en">economic entity</rdfs:label>
        <rdfs:label xml:lang="fr">entité économique</rdfs:label>
    </owl:Class>
    


    <!-- https://www.wikidata.org/wiki/Q1301433 -->

    <owl:Class rdf:about="https://www.wikidata.org/wiki/Q1301433">
        <rdfs:subClassOf rdf:resource="https://www.wikidata.org/wiki/Q42889"/>
        <rdfs:comment xml:lang="de">Fahrzeug, das sich auf festem Grund fortbewegt</rdfs:comment>
        <rdfs:comment xml:lang="en">vehicle mainly meant to move on land, including wheeled, tracked, and walking vehicles</rdfs:comment>
        <rdfs:comment xml:lang="fr">véhicule conçu pour évoluer sur la surface terrestre</rdfs:comment>
        <rdfs:label xml:lang="de">Landfahrzeug</rdfs:label>
        <rdfs:label xml:lang="en">land vehicle</rdfs:label>
        <rdfs:label xml:lang="fr">véhicule terrestre</rdfs:label>
    </owl:Class>
    


    <!-- https://www.wikidata.org/wiki/Q1308737 -->

    <owl:Class rdf:about="https://www.wikidata.org/wiki/Q1308737">
        <rdfs:subClassOf rdf:resource="https://www.wikidata.org/wiki/Q42889"/>
        <rdfs:comment xml:lang="de">speziell ausgerüstete Fahrzeuge einer Hilfsorganisation oder einer Behörde</rdfs:comment>
        <rdfs:comment xml:lang="fr">type de véhicule</rdfs:comment>
        <rdfs:comment xml:lang="en">vehicle that is designated and authorized to respond to an emergency</rdfs:comment>
        <rdfs:label xml:lang="de">Einsatzfahrzeug</rdfs:label>
        <rdfs:label xml:lang="en">emergency vehicle</rdfs:label>
        <rdfs:label xml:lang="fr">véhicule de secours</rdfs:label>
    </owl:Class>
    


    <!-- https://www.wikidata.org/wiki/Q1308813 -->

    <owl:Class rdf:about="https://www.wikidata.org/wiki/Q1308813">
        <rdfs:subClassOf rdf:resource="https://www.wikidata.org/wiki/Q1308737"/>
        <rdfs:comment xml:lang="de">Einsatzfahrzeug zu Koordinierung des Einsatzes der Feuerwehr, der THW und der Polizei</rdfs:comment>
        <rdfs:comment xml:lang="en">emergency vehicle to coordinate fire, ambulance, police, and technical operations</rdfs:comment>
        <rdfs:label xml:lang="de">Einsatzleitwagen</rdfs:label>
        <rdfs:label xml:lang="fr">Véhicule poste de commandement</rdfs:label>
        <rdfs:label xml:lang="en">emergency service command vehicle</rdfs:label>
    </owl:Class>
    


    <!-- https://www.wikidata.org/wiki/Q131085629 -->

    <owl:Class rdf:about="https://www.wikidata.org/wiki/Q131085629">
        <rdfs:subClassOf rdf:resource="https://www.wikidata.org/wiki/Q24229398"/>
        <rdfs:comment xml:lang="fr">agent qui est un groupement ou une association de deux ou plusieurs personnes portant un nom particulier et disposant de la faculté d’agir collectivement</rdfs:comment>
        <rdfs:comment xml:lang="en">an agent who is a gathering or organization of two or more persons that bears a particular name and that is capable of acting as a unit</rdfs:comment>
        <rdfs:comment xml:lang="de">ein Akteur, bei dem es sich um eine Zusammenkunft oder eine Organisation von zwei oder mehreren Personen handelt, die der einen bestimmten Namen trägt und imstande ist, als Einheit zu handeln</rdfs:comment>
        <rdfs:label xml:lang="de">Gemeinschaftlicher Akteur</rdfs:label>
        <rdfs:label xml:lang="fr">agent collectif</rdfs:label>
        <rdfs:label xml:lang="en">collective agent</rdfs:label>
    </owl:Class>
    


    <!-- https://www.wikidata.org/wiki/Q1411945 -->

    <owl:Class rdf:about="https://www.wikidata.org/wiki/Q1411945">
        <rdfs:subClassOf rdf:resource="https://www.wikidata.org/wiki/Q811979"/>
        <rdfs:comment xml:lang="de">Bauwerk mit komplexer Baustatik</rdfs:comment>
        <rdfs:comment xml:lang="fr">construction civile</rdfs:comment>
        <rdfs:comment xml:lang="en">type of construction</rdfs:comment>
        <rdfs:label xml:lang="de">Ingenieurbauwerk</rdfs:label>
        <rdfs:label xml:lang="en">civil engineering construction</rdfs:label>
        <rdfs:label xml:lang="fr">ouvrage d&apos;art</rdfs:label>
    </owl:Class>
    


    <!-- https://www.wikidata.org/wiki/Q14524070 -->

    <owl:Class rdf:about="https://www.wikidata.org/wiki/Q14524070">
        <rdfs:subClassOf rdf:resource="https://www.wikidata.org/wiki/Q1411945"/>
        <rdfs:comment xml:lang="de">Hebevorrichtung für Wasser</rdfs:comment>
        <rdfs:comment xml:lang="en">acility which is part of a water supply network and is used to transport water up an incline</rdfs:comment>
        <rdfs:label xml:lang="de">Schöpfwerk</rdfs:label>
        <rdfs:label xml:lang="fr">station de pompage des eaux</rdfs:label>
        <rdfs:label xml:lang="en">water pumping station</rdfs:label>
    </owl:Class>
    


    <!-- https://www.wikidata.org/wiki/Q1515493 -->

    <owl:Class rdf:about="https://www.wikidata.org/wiki/Q1515493">
        <rdfs:subClassOf rdf:resource="https://www.wikidata.org/wiki/Q1301433"/>
        <rdfs:comment xml:lang="de">Landfahrzeug, das vorrangig für den Betrieb auf Straßen vorgesehen ist</rdfs:comment>
        <rdfs:comment xml:lang="en">vehicle intended to be used on public streets and highways</rdfs:comment>
        <rdfs:comment xml:lang="fr">véhicule conçu pour évoluer sur routes</rdfs:comment>
        <rdfs:label xml:lang="de">Straßenfahrzeug</rdfs:label>
        <rdfs:label xml:lang="en">road vehicle</rdfs:label>
        <rdfs:label xml:lang="fr">véhicule routier</rdfs:label>
    </owl:Class>
    


    <!-- https://www.wikidata.org/wiki/Q1515989 -->

    <owl:Class rdf:about="https://www.wikidata.org/wiki/Q1515989">
        <rdfs:subClassOf rdf:resource="https://www.wikidata.org/wiki/Q1308737"/>
        <rdfs:comment xml:lang="de">spezielle Fahrzeuge der Hilfsorganisationen in Deutschland</rdfs:comment>
        <rdfs:label xml:lang="de">Gerätewagen</rdfs:label>
        <rdfs:label xml:lang="en">Gerätewagen</rdfs:label>
    </owl:Class>
    


    <!-- https://www.wikidata.org/wiki/Q155076 -->

    <owl:Class rdf:about="https://www.wikidata.org/wiki/Q155076">
        <rdfs:subClassOf rdf:resource="https://www.wikidata.org/wiki/Q3778211"/>
        <rdfs:comment xml:lang="de">Träger von Rechten oder Pflichten</rdfs:comment>
        <rdfs:comment xml:lang="fr">concept en droit</rdfs:comment>
        <rdfs:comment xml:lang="en">organization recognized by law as a fictitious person</rdfs:comment>
        <rdfs:label xml:lang="en">juridical person</rdfs:label>
        <rdfs:label xml:lang="de">juristische Person</rdfs:label>
        <rdfs:label xml:lang="fr">personne morale</rdfs:label>
    </owl:Class>
    


    <!-- https://www.wikidata.org/wiki/Q15848142 -->

    <owl:Class rdf:about="https://www.wikidata.org/wiki/Q15848142">
        <rdfs:subClassOf rdf:resource="https://www.wikidata.org/wiki/Q2466889"/>
        <rdfs:comment xml:lang="de">Bauwerk, um Binnenland vor Hochwasser zu schützen</rdfs:comment>
        <rdfs:comment xml:lang="en">hydraulic structure used to prevent tidal flooding</rdfs:comment>
        <rdfs:label xml:lang="de">Sperrwerk</rdfs:label>
        <rdfs:label xml:lang="en">Tidal barrier</rdfs:label>
        <rdfs:label xml:lang="fr">barrière contre les inondations</rdfs:label>
    </owl:Class>
    


    <!-- https://www.wikidata.org/wiki/Q16334295 -->

    <owl:Class rdf:about="https://www.wikidata.org/wiki/Q16334295">
        <rdfs:subClassOf rdf:resource="https://www.wikidata.org/wiki/Q16887380"/>
        <rdfs:comment xml:lang="en">any set of human beings</rdfs:comment>
        <rdfs:comment xml:lang="de">mehrere Menschen</rdfs:comment>
        <rdfs:comment xml:lang="fr">n&apos;importe quel groupe constitué d&apos;êtres humains</rdfs:comment>
        <rdfs:label xml:lang="de">Gruppe von Menschen</rdfs:label>
        <rdfs:label xml:lang="en">group of humans</rdfs:label>
        <rdfs:label xml:lang="fr">groupe d&apos;humains</rdfs:label>
    </owl:Class>
    


    <!-- https://www.wikidata.org/wiki/Q1633677 -->

    <owl:Class rdf:about="https://www.wikidata.org/wiki/Q1633677">
        <rdfs:subClassOf rdf:resource="https://www.wikidata.org/wiki/Q208281"/>
        <rdfs:comment xml:lang="de">Fahrzeug zur Menschenrettung aus großer höhe</rdfs:comment>
        <rdfs:label xml:lang="de">Hubrettungsfahrzeug</rdfs:label>
    </owl:Class>
    


    <!-- https://www.wikidata.org/wiki/Q16391167 -->

    <owl:Class rdf:about="https://www.wikidata.org/wiki/Q16391167">
        <rdfs:subClassOf rdf:resource="https://www.wikidata.org/wiki/Q42889"/>
        <rdfs:comment xml:lang="en">craft designed for transportation on or through air, water, or space</rdfs:comment>
        <rdfs:comment xml:lang="fr">grand véhicule</rdfs:comment>
        <rdfs:comment xml:lang="de">großes Landfahrzeug, Wasserfahrzeug, Boot, Raumschiff oder Schiff</rdfs:comment>
        <rdfs:label xml:lang="de">großes Fahrzeug</rdfs:label>
        <rdfs:label xml:lang="fr">vaisseau</rdfs:label>
        <rdfs:label xml:lang="en">vessel</rdfs:label>
    </owl:Class>
    


    <!-- https://www.wikidata.org/wiki/Q1639378 -->

    <owl:Class rdf:about="https://www.wikidata.org/wiki/Q1639378">
        <rdfs:subClassOf rdf:resource="https://www.wikidata.org/wiki/Q58778"/>
        <rdfs:comment xml:lang="de">Begriff der soziologischen Systemtheorie</rdfs:comment>
        <rdfs:comment xml:lang="en">patterned series of interrelationships existing between individuals, groups, and institutions</rdfs:comment>
        <rdfs:comment xml:lang="fr">terme principal en théorie de systèmes sociologiques</rdfs:comment>
        <rdfs:label xml:lang="en">social system</rdfs:label>
        <rdfs:label xml:lang="de">soziales System</rdfs:label>
        <rdfs:label xml:lang="fr">système social</rdfs:label>
    </owl:Class>
    


    <!-- https://www.wikidata.org/wiki/Q1656682 -->

    <owl:Class rdf:about="https://www.wikidata.org/wiki/Q1656682">
        <rdfs:subClassOf rdf:resource="https://www.wikidata.org/wiki/Q1190554"/>
        <rdfs:comment xml:lang="en">temporary and scheduled happening, like a conference, festival, competition or similar</rdfs:comment>
        <rdfs:comment xml:lang="de">zeitlich begrenztes und geplantes Ereignis, wie eine Konferenz, ein Festival, ein Wettbewerb oder ähnliches</rdfs:comment>
        <rdfs:comment xml:lang="fr">événement temporaire ou prévu, comme un festival ou une compétition</rdfs:comment>
        <rdfs:label xml:lang="de">Veranstaltung</rdfs:label>
        <rdfs:label xml:lang="en">event</rdfs:label>
        <rdfs:label xml:lang="fr">événement</rdfs:label>
    </owl:Class>
    


    <!-- https://www.wikidata.org/wiki/Q16686448 -->

    <owl:Class rdf:about="https://www.wikidata.org/wiki/Q16686448">
        <rdfs:subClassOf rdf:resource="http://purl.obolibrary.org/obo/BFO_0000030"/>
        <rdfs:comment xml:lang="en">anything created by humans (either material or mental)</rdfs:comment>
        <rdfs:comment xml:lang="fr">objet matériel ou concept créé par des humains</rdfs:comment>
        <rdfs:comment xml:lang="de">von Menschen Erschaffenes</rdfs:comment>
        <rdfs:label xml:lang="en">artificial object</rdfs:label>
        <rdfs:label xml:lang="fr">entité artificielle</rdfs:label>
        <rdfs:label xml:lang="de">künstliche Entität</rdfs:label>
    </owl:Class>
    


    <!-- https://www.wikidata.org/wiki/Q167037 -->

    <owl:Class rdf:about="https://www.wikidata.org/wiki/Q167037">
        <rdfs:subClassOf rdf:resource="https://www.wikidata.org/wiki/Q155076"/>
        <rdfs:subClassOf rdf:resource="https://www.wikidata.org/wiki/Q783794"/>
        <rdfs:comment xml:lang="de">Vereinigung, deren Bestand vom Wechsel der Mitglieder unabhängig ist</rdfs:comment>
        <rdfs:comment xml:lang="fr">legal entity incorporated through a legislative or registration process</rdfs:comment>
        <rdfs:comment xml:lang="fr">réunion durable de personnes poursuivant un but commun</rdfs:comment>
        <rdfs:label xml:lang="de">Körperschaft</rdfs:label>
        <rdfs:label xml:lang="en">corporation</rdfs:label>
        <rdfs:label xml:lang="fr">corporation</rdfs:label>
    </owl:Class>
    


    <!-- https://www.wikidata.org/wiki/Q16887380 -->

    <owl:Class rdf:about="https://www.wikidata.org/wiki/Q16887380">
        <rdfs:subClassOf rdf:resource="https://www.wikidata.org/wiki/Q28813620"/>
        <rdfs:comment xml:lang="de">fasst Entitäten mit ähnlichen Eigenschaften zusammen</rdfs:comment>
        <rdfs:comment xml:lang="fr">regroupement d&apos;entités discrètes qui ont choisi ou ont été affectés à un tout</rdfs:comment>
        <rdfs:comment xml:lang="en">well-defined, enumerable collection of discrete entities that form a collective whole</rdfs:comment>
        <rdfs:label xml:lang="de">Gruppe</rdfs:label>
        <rdfs:label xml:lang="en">group</rdfs:label>
        <rdfs:label xml:lang="fr">groupe</rdfs:label>
    </owl:Class>
    


    <!-- https://www.wikidata.org/wiki/Q1882685 -->

    <owl:Class rdf:about="https://www.wikidata.org/wiki/Q1882685">
        <rdfs:subClassOf rdf:resource="https://www.wikidata.org/wiki/Q11019"/>
        <rdfs:comment xml:lang="en">device employing power to achieve desired forces and/or motion</rdfs:comment>
        <rdfs:label xml:lang="en">mechanical device</rdfs:label>
        <rdfs:label xml:lang="de">mechanisches Gerät</rdfs:label>
    </owl:Class>
    


    <!-- https://www.wikidata.org/wiki/Q1898202 -->

    <owl:Class rdf:about="https://www.wikidata.org/wiki/Q1898202">
        <rdfs:subClassOf rdf:resource="https://www.wikidata.org/wiki/Q1633677"/>
        <rdfs:comment xml:lang="de">Hubrettungsfahrzeug der Feuerwehr</rdfs:comment>
        <rdfs:comment xml:lang="en">type of fire engine</rdfs:comment>
        <rdfs:comment xml:lang="fr">véhicule des pompiers qui emporte une échelle escamotable de grande hauteur</rdfs:comment>
        <rdfs:label xml:lang="de">Drehleiter</rdfs:label>
        <rdfs:label xml:lang="en">turntable ladder</rdfs:label>
        <rdfs:label xml:lang="fr">échelle pivotante automatique</rdfs:label>
    </owl:Class>
    


    <!-- https://www.wikidata.org/wiki/Q1914636 -->

    <owl:Class rdf:about="https://www.wikidata.org/wiki/Q1914636">
        <rdfs:subClassOf rdf:resource="https://www.wikidata.org/wiki/Q3249551"/>
        <rdfs:comment xml:lang="de">Handeln, kann sowohl körperliche als auch geistige Verrichtungen umfassen</rdfs:comment>
        <rdfs:comment xml:lang="fr">action de faire quelque chose</rdfs:comment>
        <rdfs:comment xml:lang="en">series of actions done by an agent which results in an external change of state</rdfs:comment>
        <rdfs:label xml:lang="de">Tätigkeit</rdfs:label>
        <rdfs:label xml:lang="en">activity</rdfs:label>
        <rdfs:label xml:lang="fr">activité</rdfs:label>
    </owl:Class>
    


    <!-- https://www.wikidata.org/wiki/Q193078 -->

    <owl:Class rdf:about="https://www.wikidata.org/wiki/Q193078">
        <rdfs:subClassOf rdf:resource="https://www.wikidata.org/wiki/Q117134054"/>
        <rdfs:comment xml:lang="de">Schädigung, Verletzung oder Verwundung, die durch Gewalt von außen entsteht</rdfs:comment>
        <rdfs:comment xml:lang="fr">dommage ou choc provoqué par une blessure physique</rdfs:comment>
        <rdfs:comment xml:lang="en">physiological wound caused by an external source</rdfs:comment>
        <rdfs:label xml:lang="de">Trauma</rdfs:label>
        <rdfs:label xml:lang="en">injury in humans</rdfs:label>
        <rdfs:label xml:lang="fr">traumatisme</rdfs:label>
    </owl:Class>
    


    <!-- https://www.wikidata.org/wiki/Q208281 -->

    <owl:Class rdf:about="https://www.wikidata.org/wiki/Q208281">
        <rdfs:subClassOf rdf:resource="https://www.wikidata.org/wiki/Q1515493"/>
        <rdfs:comment xml:lang="de">Fahrzeug mit Sonderausstattung zum Löschen von Bränden für die Feuerwehr</rdfs:comment>
        <rdfs:comment xml:lang="fr">camion de pompiers utilisé dans la lutte contre l&apos;incendie</rdfs:comment>
        <rdfs:comment xml:lang="en">emergency ground vehicle intended to put out fires</rdfs:comment>
        <rdfs:label xml:lang="de">Feuerwehrfahrzeug</rdfs:label>
        <rdfs:label xml:lang="en">fire engine</rdfs:label>
        <rdfs:label xml:lang="fr">fourgon d&apos;incendie</rdfs:label>
    </owl:Class>
    


    <!-- https://www.wikidata.org/wiki/Q216146 -->

    <owl:Class rdf:about="https://www.wikidata.org/wiki/Q216146">
        <rdfs:subClassOf rdf:resource="https://www.wikidata.org/wiki/Q1301433"/>
        <rdfs:comment xml:lang="de">Fahrzeug, das über eine Ladefläche, jedoch keinen eigenen Antrieb verfügt</rdfs:comment>
        <rdfs:comment xml:lang="en">vehicle that has a loading area but does not have its own propulsion</rdfs:comment>
        <rdfs:comment xml:lang="fr">véhicule qui a une zone de chargement, mais pas de moteur</rdfs:comment>
        <rdfs:label xml:lang="de">Anhänger</rdfs:label>
        <rdfs:label xml:lang="fr">remorque</rdfs:label>
        <rdfs:label xml:lang="en">trailer</rdfs:label>
    </owl:Class>
    


    <!-- https://www.wikidata.org/wiki/Q223557 -->

    <owl:Class rdf:about="https://www.wikidata.org/wiki/Q223557">
        <rdfs:subClassOf rdf:resource="https://www.wikidata.org/wiki/Q4406616"/>
        <rdfs:comment xml:lang="de">Ansammlung von Masse, die eine Einheit bildet</rdfs:comment>
        <rdfs:comment xml:lang="fr">agrégation singulière de substance(s) tangibles comme des matières ou des radiations, avec des propriétés globales</rdfs:comment>
        <rdfs:comment xml:lang="en">singular aggregation of substance(s) such as matter or radiation, with overall properties such as mass, position or momentum</rdfs:comment>
        <rdfs:label xml:lang="de">Körper</rdfs:label>
        <rdfs:label xml:lang="fr">objet physique</rdfs:label>
        <rdfs:label xml:lang="en">physical object</rdfs:label>
    </owl:Class>
    


    <!-- https://www.wikidata.org/wiki/Q22445448 -->

    <owl:Class rdf:about="https://www.wikidata.org/wiki/Q22445448">
        <rdfs:subClassOf rdf:resource="https://www.wikidata.org/wiki/Q1190554"/>
        <rdfs:comment xml:lang="en">act of asking politely or formally for something</rdfs:comment>
        <rdfs:comment xml:lang="de">höflich ausgedrückter Wunsch</rdfs:comment>
        <rdfs:label xml:lang="de">Bitte</rdfs:label>
        <rdfs:label xml:lang="fr">demande</rdfs:label>
        <rdfs:label xml:lang="en">request</rdfs:label>
    </owl:Class>
    


    <!-- https://www.wikidata.org/wiki/Q2345125 -->

    <owl:Class rdf:about="https://www.wikidata.org/wiki/Q2345125">
        <rdfs:subClassOf rdf:resource="https://www.wikidata.org/wiki/Q105731"/>
        <rdfs:comment xml:lang="en">adjustable gate used to control water flow</rdfs:comment>
        <rdfs:comment xml:lang="de">bewegliches Schott zum Absperren eines niederen Wasserstandes</rdfs:comment>
        <rdfs:label xml:lang="de">Fluttor</rdfs:label>
        <rdfs:label xml:lang="en">floodgate</rdfs:label>
        <rdfs:label xml:lang="fr">vanne contre les inondations</rdfs:label>
    </owl:Class>
    


    <!-- https://www.wikidata.org/wiki/Q23580581 -->

    <owl:Class rdf:about="https://www.wikidata.org/wiki/Q23580581">
        <rdfs:subClassOf rdf:resource="https://www.wikidata.org/wiki/Q61788060"/>
        <rdfs:comment xml:lang="en">losing spatial reference</rdfs:comment>
        <rdfs:label xml:lang="de">Verirren</rdfs:label>
        <rdfs:label xml:lang="en">getting lost</rdfs:label>
    </owl:Class>
    


    <!-- https://www.wikidata.org/wiki/Q24229398 -->

    <owl:Class rdf:about="https://www.wikidata.org/wiki/Q24229398">
        <rdfs:subClassOf rdf:resource="http://purl.obolibrary.org/obo/BFO_0000004"/>
        <rdfs:comment xml:lang="de">Entität, die Aktionen ausführen kann</rdfs:comment>
        <rdfs:comment xml:lang="en">distinct and identifiable entity capable of performing actions</rdfs:comment>
        <rdfs:comment xml:lang="fr">entité individuelle et identifiable qui peut conduire des actions (comme une personne physique ou une organisation)</rdfs:comment>
        <rdfs:label xml:lang="de">Akteur</rdfs:label>
        <rdfs:label xml:lang="en">agent</rdfs:label>
        <rdfs:label xml:lang="fr">agent</rdfs:label>
    </owl:Class>
    


    <!-- https://www.wikidata.org/wiki/Q2466889 -->

    <owl:Class rdf:about="https://www.wikidata.org/wiki/Q2466889">
        <rdfs:subClassOf rdf:resource="https://www.wikidata.org/wiki/Q1411945"/>
        <rdfs:subClassOf rdf:resource="https://www.wikidata.org/wiki/Q811979"/>
        <rdfs:comment xml:lang="de">Bauwerk, das einen natürlichen Wasserlauf verändert</rdfs:comment>
        <rdfs:comment xml:lang="en">artificial structure which disrupts the natural flow of water</rdfs:comment>
        <rdfs:comment xml:lang="fr">type d&apos;ouvrage d&apos;art</rdfs:comment>
        <rdfs:label xml:lang="en">hydraulic structure</rdfs:label>
        <rdfs:label xml:lang="de">hydraulisches Bauwerk</rdfs:label>
        <rdfs:label xml:lang="fr">ouvrage hydraulique</rdfs:label>
    </owl:Class>
    


    <!-- https://www.wikidata.org/wiki/Q27096213 -->

    <owl:Class rdf:about="https://www.wikidata.org/wiki/Q27096213">
        <rdfs:subClassOf rdf:resource="https://www.wikidata.org/wiki/Q123349660"/>
        <rdfs:comment xml:lang="de">Ort oder Objekt</rdfs:comment>
        <rdfs:comment xml:lang="fr">lieu ou entité susceptible de l&apos;être</rdfs:comment>
        <rdfs:comment xml:lang="en">relatively stationary place or entity that can be geographically identified, located, or described</rdfs:comment>
        <rdfs:label xml:lang="fr">entité géographique</rdfs:label>
        <rdfs:label xml:lang="de">geografische Entität</rdfs:label>
        <rdfs:label xml:lang="en">geographic entity</rdfs:label>
    </owl:Class>
    


    <!-- https://www.wikidata.org/wiki/Q286897 -->

    <owl:Class rdf:about="https://www.wikidata.org/wiki/Q286897">
        <rdfs:subClassOf rdf:resource="https://www.wikidata.org/wiki/Q1515989"/>
        <rdfs:label xml:lang="de">Messfahrzeug</rdfs:label>
    </owl:Class>
    


    <!-- https://www.wikidata.org/wiki/Q28813620 -->

    <owl:Class rdf:about="https://www.wikidata.org/wiki/Q28813620">
        <rdfs:subClassOf rdf:resource="https://www.wikidata.org/wiki/Q99527517"/>
        <rdfs:comment xml:lang="de">Gruppe von Dingen</rdfs:comment>
        <rdfs:comment xml:lang="fr">ensemble d&apos;éléments tenus individuellement ; analogue à un ensemble mathématique, mais permettant aussi des éléments non mathématiques</rdfs:comment>
        <rdfs:comment xml:lang="en">group of items regarded as one</rdfs:comment>
        <rdfs:label xml:lang="de">Gefüge</rdfs:label>
        <rdfs:label xml:lang="fr">ensemble</rdfs:label>
        <rdfs:label xml:lang="en">set</rdfs:label>
    </owl:Class>
    


    <!-- https://www.wikidata.org/wiki/Q3249551 -->

    <owl:Class rdf:about="https://www.wikidata.org/wiki/Q3249551">
        <rdfs:subClassOf rdf:resource="http://purl.obolibrary.org/obo/BFO_0000003"/>
        <rdfs:comment xml:lang="de">Folge von Änderungen</rdfs:comment>
        <rdfs:comment xml:lang="en">series of events which occur over an extended period of time</rdfs:comment>
        <rdfs:comment xml:lang="fr">série d&apos;événements qui surviennent sur une période de temps étendue</rdfs:comment>
        <rdfs:label xml:lang="de">Vorgang</rdfs:label>
        <rdfs:label xml:lang="en">process</rdfs:label>
        <rdfs:label xml:lang="fr">processus</rdfs:label>
    </owl:Class>
    


    <!-- https://www.wikidata.org/wiki/Q333170 -->

    <owl:Class rdf:about="https://www.wikidata.org/wiki/Q333170">
        <rdfs:subClassOf rdf:resource="https://www.wikidata.org/wiki/Q107589046"/>
        <rdfs:comment xml:lang="de">Verkehrswasserbauwerk, das Wasserfahrzeugen das Überwinden eines Höhenunterschiedes ermöglicht</rdfs:comment>
        <rdfs:comment xml:lang="en">structure that allows vessels to overcome a fall in a waterway</rdfs:comment>
        <rdfs:label xml:lang="de">Abstiegsbauwerk</rdfs:label>
        <rdfs:label xml:lang="en">fall structure</rdfs:label>
    </owl:Class>
    


    <!-- https://www.wikidata.org/wiki/Q37112258 -->

    <owl:Class rdf:about="https://www.wikidata.org/wiki/Q37112258">
        <rdfs:subClassOf rdf:resource="https://www.wikidata.org/wiki/Q1914636"/>
        <rdfs:comment xml:lang="en">event of locating or identifying something</rdfs:comment>
        <rdfs:comment xml:lang="fr">fait de localiser ou d&apos;identifier quelque chose</rdfs:comment>
        <rdfs:label xml:lang="de">Finden</rdfs:label>
        <rdfs:label xml:lang="fr">découverte</rdfs:label>
        <rdfs:label xml:lang="en">finding</rdfs:label>
    </owl:Class>
    


    <!-- https://www.wikidata.org/wiki/Q3778211 -->

    <owl:Class rdf:about="https://www.wikidata.org/wiki/Q3778211">
        <rdfs:subClassOf rdf:resource="https://www.wikidata.org/wiki/Q106559804"/>
        <rdfs:comment xml:lang="de">Träger von (subjektiven) Rechten und Rechtspflichten</rdfs:comment>
        <rdfs:comment xml:lang="en">any human or non-human entity that is recognized as having privileges and obligations; a legal fiction which is used to abstract away the differences between natural persons, juridical persons and other entities such as countries</rdfs:comment>
        <rdfs:comment xml:lang="fr">aptitude à être titulaire de droits et de devoirs</rdfs:comment>
        <rdfs:label xml:lang="de">Rechtssubjekt</rdfs:label>
        <rdfs:label xml:lang="en">legal person</rdfs:label>
        <rdfs:label xml:lang="fr">personnalité juridique</rdfs:label>
    </owl:Class>
    


    <!-- https://www.wikidata.org/wiki/Q39546 -->

    <owl:Class rdf:about="https://www.wikidata.org/wiki/Q39546">
        <rdfs:subClassOf rdf:resource="https://www.wikidata.org/wiki/Q10273457"/>
        <rdfs:subClassOf rdf:resource="https://www.wikidata.org/wiki/Q123691918"/>
        <rdfs:subClassOf rdf:resource="https://www.wikidata.org/wiki/Q8205328"/>
        <rdfs:comment xml:lang="de">Arbeitsmittel, um auf Gegenstände einzuwirken</rdfs:comment>
        <rdfs:comment xml:lang="fr">instrument physique utilisable pour exercer une action</rdfs:comment>
        <rdfs:comment xml:lang="en">physical item that can be used to achieve a goal</rdfs:comment>
        <rdfs:label xml:lang="de">Werkzeug</rdfs:label>
        <rdfs:label xml:lang="fr">outil</rdfs:label>
        <rdfs:label xml:lang="en">physical tool</rdfs:label>
    </owl:Class>
    


    <!-- https://www.wikidata.org/wiki/Q4 -->

    <owl:Class rdf:about="https://www.wikidata.org/wiki/Q4">
        <rdfs:subClassOf rdf:resource="https://www.wikidata.org/wiki/Q1190554"/>
        <rdfs:comment xml:lang="de">endgültiger Verlust der Lebensfunktionen</rdfs:comment>
        <rdfs:comment xml:lang="en">permanent cessation of vital functions</rdfs:comment>
        <rdfs:comment xml:lang="fr">état de ce dont les fonctions vitales se sont arrêtées</rdfs:comment>
        <rdfs:label xml:lang="de">Tod</rdfs:label>
        <rdfs:label xml:lang="en">death</rdfs:label>
        <rdfs:label xml:lang="fr">mort</rdfs:label>
    </owl:Class>
    


    <!-- https://www.wikidata.org/wiki/Q4026292 -->

    <owl:Class rdf:about="https://www.wikidata.org/wiki/Q4026292">
        <rdfs:subClassOf rdf:resource="https://www.wikidata.org/wiki/Q1190554"/>
        <rdfs:comment xml:lang="de">absichtliche Tätigkeiten eines Menschen</rdfs:comment>
        <rdfs:comment xml:lang="fr">ce qui peut être fait par un agent</rdfs:comment>
        <rdfs:comment xml:lang="en">something an agent can do or perform</rdfs:comment>
        <rdfs:label xml:lang="de">Handeln</rdfs:label>
        <rdfs:label xml:lang="en">action</rdfs:label>
        <rdfs:label xml:lang="fr">action</rdfs:label>
    </owl:Class>
    


    <!-- https://www.wikidata.org/wiki/Q42889 -->

    <owl:Class rdf:about="https://www.wikidata.org/wiki/Q42889">
        <rdfs:subClassOf rdf:resource="https://www.wikidata.org/wiki/Q106839123"/>
        <rdfs:subClassOf rdf:resource="https://www.wikidata.org/wiki/Q11019"/>
        <rdfs:comment xml:lang="fr">machine mobile qui transporte, qu&apos;elle soit motorisée ou non, telle qu&apos;un vélo, une voiture, un autre véhicule terrestre (y compris les véhicules à roues et à chenilles), un aéronef ou une embarcation</rdfs:comment>
        <rdfs:comment xml:lang="en">mobile machine used for transport, whether it has an engine or not, including wheeled and tracked vehicles, air-, water-, and space-craft</rdfs:comment>
        <rdfs:comment xml:lang="de">mobiles Transportmittel</rdfs:comment>
        <rdfs:label xml:lang="de">Verkehrsmittel</rdfs:label>
        <rdfs:label xml:lang="en">vehicle</rdfs:label>
        <rdfs:label xml:lang="fr">véhicule</rdfs:label>
    </owl:Class>
    


    <!-- https://www.wikidata.org/wiki/Q43229 -->

    <owl:Class rdf:about="https://www.wikidata.org/wiki/Q43229">
        <rdfs:subClassOf rdf:resource="https://www.wikidata.org/wiki/Q106559804"/>
        <rdfs:subClassOf rdf:resource="https://www.wikidata.org/wiki/Q106668099"/>
        <rdfs:subClassOf rdf:resource="https://www.wikidata.org/wiki/Q16334295"/>
        <rdfs:subClassOf rdf:resource="https://www.wikidata.org/wiki/Q1639378"/>
        <rdfs:subClassOf rdf:resource="https://www.wikidata.org/wiki/Q854457"/>
        <rdfs:comment xml:lang="fr">entité sociale (non nécessairement commerciale) réunissant des personnes en un groupe structuré gérant des moyens communs pour répondre à certains besoins ou poursuivre des objectifs collectifs</rdfs:comment>
        <rdfs:comment xml:lang="en">social entity established to meet needs or pursue goals</rdfs:comment>
        <rdfs:comment xml:lang="de">soziale Struktur mit einem gemeinsamen Ziel</rdfs:comment>
        <rdfs:label xml:lang="de">Organisation</rdfs:label>
        <rdfs:label xml:lang="fr">organisation</rdfs:label>
        <rdfs:label xml:lang="en">organization</rdfs:label>
    </owl:Class>
    


    <!-- https://www.wikidata.org/wiki/Q4406616 -->

    <owl:Class rdf:about="https://www.wikidata.org/wiki/Q4406616">
        <rdfs:subClassOf rdf:resource="http://purl.obolibrary.org/obo/BFO_0000030"/>
        <rdfs:comment xml:lang="en">a particular or specific instance of an entity</rdfs:comment>
        <rdfs:comment xml:lang="de">etwas mit einer physikalischen Manifestation</rdfs:comment>
        <rdfs:comment xml:lang="fr">objet ayant une manifestation physique</rdfs:comment>
        <rdfs:label xml:lang="en">concrete object</rdfs:label>
        <rdfs:label xml:lang="de">konkretes Objekt</rdfs:label>
        <rdfs:label xml:lang="fr">objet concret</rdfs:label>
    </owl:Class>
    


    <!-- https://www.wikidata.org/wiki/Q446013 -->

    <owl:Class rdf:about="https://www.wikidata.org/wiki/Q446013">
        <rdfs:subClassOf rdf:resource="https://www.wikidata.org/wiki/Q2466889"/>
        <rdfs:comment xml:lang="de">Anlage, mit der Wasser aus einem niedriger gelegenen Gewässer in ein höher gelegenes gepumpt wird</rdfs:comment>
        <rdfs:comment xml:lang="en">facilities including pumps and equipment for pumping fluids from one place to another</rdfs:comment>
        <rdfs:label xml:lang="de">Pumpwerk</rdfs:label>
        <rdfs:label xml:lang="en">pumping station</rdfs:label>
        <rdfs:label xml:lang="fr">station de pompage</rdfs:label>
    </owl:Class>
    


    <!-- https://www.wikidata.org/wiki/Q451967 -->

    <owl:Class rdf:about="https://www.wikidata.org/wiki/Q451967">
        <rdfs:subClassOf rdf:resource="https://www.wikidata.org/wiki/Q61788060"/>
        <rdfs:comment xml:lang="fr">activité humaine basée sur un motif quelconque</rdfs:comment>
        <rdfs:comment xml:lang="en">human activity driven by purposeful motives</rdfs:comment>
        <rdfs:comment xml:lang="de">jede menschliche, von Motiven geleitete zielgerichtete Aktivität</rdfs:comment>
        <rdfs:label xml:lang="fr">action humaine</rdfs:label>
        <rdfs:label xml:lang="en">intentional human activity</rdfs:label>
        <rdfs:label xml:lang="de">menschliche Handlung</rdfs:label>
    </owl:Class>
    


    <!-- https://www.wikidata.org/wiki/Q47496130 -->

    <owl:Class rdf:about="https://www.wikidata.org/wiki/Q47496130">
        <rdfs:subClassOf rdf:resource="https://www.wikidata.org/wiki/Q1150070"/>
        <rdfs:comment xml:lang="en">decrease in a quantity</rdfs:comment>
        <rdfs:comment xml:lang="fr">réduction d&apos;une quantité</rdfs:comment>
        <rdfs:label xml:lang="de">Verringerung</rdfs:label>
        <rdfs:label xml:lang="fr">diminution</rdfs:label>
        <rdfs:label xml:lang="en">reduction</rdfs:label>
    </owl:Class>
    


    <!-- https://www.wikidata.org/wiki/Q481609 -->

    <owl:Class rdf:about="https://www.wikidata.org/wiki/Q481609">
        <rdfs:subClassOf rdf:resource="https://www.wikidata.org/wiki/Q3249551"/>
        <rdfs:subClassOf rdf:resource="https://www.wikidata.org/wiki/Q47496130"/>
        <rdfs:comment xml:lang="en">changes to a system that adversely affect its current or future performance</rdfs:comment>
        <rdfs:comment xml:lang="de">jeder Nachteil, den eine Person oder Sache durch ein Ereignis erleidet</rdfs:comment>
        <rdfs:comment xml:lang="fr">tout inconvénient qu&apos;une personne ou une chose souffre d&apos;un événement</rdfs:comment>
        <rdfs:label xml:lang="de">Schaden</rdfs:label>
        <rdfs:label xml:lang="en">damage</rdfs:label>
        <rdfs:label xml:lang="de">dégât</rdfs:label>
    </owl:Class>
    


    <!-- https://www.wikidata.org/wiki/Q4830453 -->

    <owl:Class rdf:about="https://www.wikidata.org/wiki/Q4830453">
        <rdfs:subClassOf rdf:resource="https://www.wikidata.org/wiki/Q12569864"/>
        <rdfs:subClassOf rdf:resource="https://www.wikidata.org/wiki/Q155076"/>
        <rdfs:subClassOf rdf:resource="https://www.wikidata.org/wiki/Q167037"/>
        <rdfs:subClassOf rdf:resource="https://www.wikidata.org/wiki/Q43229"/>
        <rdfs:comment xml:lang="fr">entité impliquée dans des activités commerciales, industrielles ou professionnelles</rdfs:comment>
        <rdfs:comment xml:lang="de">gewerbliche oder kaufmännische Geschäftseinheit</rdfs:comment>
        <rdfs:comment xml:lang="en">organization undertaking commercial, industrial, or professional activity</rdfs:comment>
        <rdfs:label xml:lang="de">Gewerbebetrieb</rdfs:label>
        <rdfs:label xml:lang="en">business</rdfs:label>
        <rdfs:label xml:lang="fr">firme</rdfs:label>
    </owl:Class>
    


    <!-- https://www.wikidata.org/wiki/Q50659049 -->

    <owl:Class rdf:about="https://www.wikidata.org/wiki/Q50659049">
        <rdfs:subClassOf rdf:resource="https://www.wikidata.org/wiki/Q1898202"/>
        <rdfs:label xml:lang="de">Drehleiter mit Korb 23/12</rdfs:label>
    </owl:Class>
    


    <!-- https://www.wikidata.org/wiki/Q510255 -->

    <owl:Class rdf:about="https://www.wikidata.org/wiki/Q510255">
        <rdfs:subClassOf rdf:resource="https://www.wikidata.org/wiki/Q107589046"/>
        <rdfs:comment xml:lang="fr">ouvrage de vidange de digue</rdfs:comment>
        <rdfs:comment xml:lang="de">verschließbarer Gewässerdurchlass in einem Deich</rdfs:comment>
        <rdfs:label xml:lang="de">Siel</rdfs:label>
        <rdfs:label xml:lang="en">discharge sluice</rdfs:label>
        <rdfs:label xml:lang="fr">écluse de chasse</rdfs:label>
    </owl:Class>
    


    <!-- https://www.wikidata.org/wiki/Q58778 -->

    <owl:Class rdf:about="https://www.wikidata.org/wiki/Q58778">
        <rdfs:subClassOf rdf:resource="http://purl.obolibrary.org/obo/BFO_0000030"/>
        <rdfs:subClassOf rdf:resource="https://www.wikidata.org/wiki/Q99527517"/>
        <rdfs:comment xml:lang="de">Gesamtheit von wechselwirkenden Elementen einer Einheit</rdfs:comment>
        <rdfs:comment xml:lang="fr">ensemble d&apos;éléments interagissant entre eux selon certains principes ou règles</rdfs:comment>
        <rdfs:comment xml:lang="en">set of interacting or interdependent components</rdfs:comment>
        <rdfs:label xml:lang="de">System</rdfs:label>
        <rdfs:label xml:lang="en">system</rdfs:label>
        <rdfs:label xml:lang="fr">système</rdfs:label>
    </owl:Class>
    


    <!-- https://www.wikidata.org/wiki/Q6056746 -->

    <owl:Class rdf:about="https://www.wikidata.org/wiki/Q6056746">
        <rdfs:subClassOf rdf:resource="https://www.wikidata.org/wiki/Q1656682"/>
        <rdfs:comment xml:lang="fr">action temporaire avec un objectif défini, qui est tenté par la coopération planifiée et coordonnée de plusieurs personnes ou acteurs</rdfs:comment>
        <rdfs:comment xml:lang="en">series of operations undertaken to achieve a defined goal</rdfs:comment>
        <rdfs:comment xml:lang="de">zeitlich befristete Aktion mit einem definierten Ziel</rdfs:comment>
        <rdfs:label xml:lang="de">Kampagne</rdfs:label>
        <rdfs:label xml:lang="fr">campagne</rdfs:label>
        <rdfs:label xml:lang="en">campaign</rdfs:label>
    </owl:Class>
    


    <!-- https://www.wikidata.org/wiki/Q606332 -->

    <owl:Class rdf:about="https://www.wikidata.org/wiki/Q606332">
        <rdfs:subClassOf rdf:resource="https://www.wikidata.org/wiki/Q11858035"/>
        <rdfs:comment xml:lang="de">Menschenansammlung bei Notfällen</rdfs:comment>
        <rdfs:comment xml:lang="fr">mouvement organisé, rapide et immédiat de personnes écartées d&apos;un danger</rdfs:comment>
        <rdfs:comment xml:lang="en">urgent movement of people away from the threat or actual occurrence of a hazard</rdfs:comment>
        <rdfs:label xml:lang="de">Evakuierung</rdfs:label>
        <rdfs:label xml:lang="en">evacuation</rdfs:label>
        <rdfs:label xml:lang="fr">évacuation</rdfs:label>
    </owl:Class>
    


    <!-- https://www.wikidata.org/wiki/Q61788060 -->

    <owl:Class rdf:about="https://www.wikidata.org/wiki/Q61788060">
        <rdfs:subClassOf rdf:resource="https://www.wikidata.org/wiki/Q1914636"/>
        <rdfs:comment xml:lang="de">Aktivität, die von Menschen praktiziert werden kann</rdfs:comment>
        <rdfs:comment xml:lang="en">activity initiated by a human, intentionally or unintentionally</rdfs:comment>
        <rdfs:comment xml:lang="fr">type d&apos;áctivité</rdfs:comment>
        <rdfs:label xml:lang="fr">activité humaine</rdfs:label>
        <rdfs:label xml:lang="en">human activity</rdfs:label>
        <rdfs:label xml:lang="de">menschliche Aktivität</rdfs:label>
    </owl:Class>
    


    <!-- https://www.wikidata.org/wiki/Q618123 -->

    <owl:Class rdf:about="https://www.wikidata.org/wiki/Q618123">
        <rdfs:subClassOf rdf:resource="https://www.wikidata.org/wiki/Q27096213"/>
        <rdfs:comment xml:lang="de">Objekt, welches mittels Geodaten eindeutig referenzierbar war bzw. ist</rdfs:comment>
        <rdfs:comment xml:lang="en">components of planets that can be geographically located</rdfs:comment>
        <rdfs:comment xml:lang="fr">entité identifiée de manière unique par une donnée spatiale</rdfs:comment>
        <rdfs:label xml:lang="en">geographical feature</rdfs:label>
        <rdfs:label xml:lang="de">geographisches Objekt</rdfs:label>
        <rdfs:label xml:lang="fr">objet géographique</rdfs:label>
    </owl:Class>
    


    <!-- https://www.wikidata.org/wiki/Q6881760 -->

    <owl:Class rdf:about="https://www.wikidata.org/wiki/Q6881760">
        <rdfs:subClassOf rdf:resource="https://www.wikidata.org/wiki/Q47496130"/>
        <rdfs:comment xml:lang="en">reduction of harm</rdfs:comment>
        <rdfs:label xml:lang="de">Folgenminderungsstrategie</rdfs:label>
        <rdfs:label xml:lang="en">mitigation</rdfs:label>
        <rdfs:label xml:lang="fr">mitigation</rdfs:label>
    </owl:Class>
    


    <!-- https://www.wikidata.org/wiki/Q7194062 -->

    <owl:Class rdf:about="https://www.wikidata.org/wiki/Q7194062">
        <rdfs:subClassOf rdf:resource="https://www.wikidata.org/wiki/Q116780996"/>
        <rdfs:subClassOf rdf:resource="https://www.wikidata.org/wiki/Q1882685"/>
        <rdfs:comment xml:lang="de">eine Maschine, die in der Luft oder im Weltall fliegen kann</rdfs:comment>
        <rdfs:comment xml:lang="fr">machine qui vole dans l&apos;air ou dans l&apos;espace</rdfs:comment>
        <rdfs:comment xml:lang="en">machine that can fly, including aircraft, spacecraft, rockets, and missiles</rdfs:comment>
        <rdfs:label xml:lang="de">Flugmaschine</rdfs:label>
        <rdfs:label xml:lang="en">flying machine</rdfs:label>
        <rdfs:label xml:lang="fr">véhicule aérospatial</rdfs:label>
    </owl:Class>
    


    <!-- https://www.wikidata.org/wiki/Q783794 -->

    <owl:Class rdf:about="https://www.wikidata.org/wiki/Q783794">
        <rdfs:subClassOf rdf:resource="https://www.wikidata.org/wiki/Q3778211"/>
        <rdfs:subClassOf rdf:resource="https://www.wikidata.org/wiki/Q43229"/>
        <rdfs:comment xml:lang="de">Zusammenschluss von mindestens zwei natürlichen und/oder juristischen Personen</rdfs:comment>
        <rdfs:comment xml:lang="fr">association de personnes individuelles réelles et/ou d&apos;autres sociétés</rdfs:comment>
        <rdfs:comment xml:lang="en">legal entity representing an association of people, whether natural, legal or a mixture of both, with a specific objective</rdfs:comment>
        <rdfs:label xml:lang="de">Gesellschaft</rdfs:label>
        <rdfs:label xml:lang="fr">compagnie</rdfs:label>
        <rdfs:label xml:lang="en">company</rdfs:label>
    </owl:Class>
    


    <!-- https://www.wikidata.org/wiki/Q811430 -->

    <owl:Class rdf:about="https://www.wikidata.org/wiki/Q811430">
        <rdfs:subClassOf rdf:resource="https://www.wikidata.org/wiki/Q618123"/>
        <rdfs:comment xml:lang="de">Konstruktion von Bauwerken und Gebäuden</rdfs:comment>
        <rdfs:comment xml:lang="en">artificially constructed entity meant to remain at a fixed geographic location</rdfs:comment>
        <rdfs:comment xml:lang="fr">objet physique</rdfs:comment>
        <rdfs:label xml:lang="de">Baukonstruktion</rdfs:label>
        <rdfs:label xml:lang="en">fixed construction</rdfs:label>
        <rdfs:label xml:lang="fr">structure construite</rdfs:label>
    </owl:Class>
    


    <!-- https://www.wikidata.org/wiki/Q811979 -->

    <owl:Class rdf:about="https://www.wikidata.org/wiki/Q811979">
        <rdfs:subClassOf rdf:resource="https://www.wikidata.org/wiki/Q811430"/>
        <rdfs:comment xml:lang="de">Konstruktion mit ruhendem Kontakt zum Untergrund, z. B. Straße, Brücke, Fundament</rdfs:comment>
        <rdfs:comment xml:lang="fr">construction dont la conception a été pensée</rdfs:comment>
        <rdfs:comment xml:lang="en">human-designed and -made structure</rdfs:comment>
        <rdfs:label xml:lang="de">Bauwerk</rdfs:label>
        <rdfs:label xml:lang="en">architectural structure</rdfs:label>
        <rdfs:label xml:lang="fr">structure architecturale</rdfs:label>
    </owl:Class>
    


    <!-- https://www.wikidata.org/wiki/Q8205328 -->

    <owl:Class rdf:about="https://www.wikidata.org/wiki/Q8205328">
        <rdfs:subClassOf rdf:resource="https://www.wikidata.org/wiki/Q16686448"/>
        <rdfs:subClassOf rdf:resource="https://www.wikidata.org/wiki/Q223557"/>
        <rdfs:comment xml:lang="de">durch menschliche oder technische Einwirkung entstandenes Produkt</rdfs:comment>
        <rdfs:comment xml:lang="fr">objet physique créé ou ayant subi une transformation par l’être humain</rdfs:comment>
        <rdfs:comment xml:lang="en">physical object made or shaped by humans</rdfs:comment>
        <rdfs:label xml:lang="de">Artefakt</rdfs:label>
        <rdfs:label xml:lang="en">artificial physical object</rdfs:label>
        <rdfs:label xml:lang="fr">objet artificiel physique</rdfs:label>
    </owl:Class>
    


    <!-- https://www.wikidata.org/wiki/Q831723 -->

    <owl:Class rdf:about="https://www.wikidata.org/wiki/Q831723">
        <rdfs:subClassOf rdf:resource="https://www.wikidata.org/wiki/Q1515989"/>
        <rdfs:comment xml:lang="de">Fahrzeug des deutschen Zivil- und Katastrophenschutzes</rdfs:comment>
        <rdfs:label xml:lang="de">Betreuungslastkraftwagen</rdfs:label>
    </owl:Class>
    


    <!-- https://www.wikidata.org/wiki/Q854457 -->

    <owl:Class rdf:about="https://www.wikidata.org/wiki/Q854457">
        <rdfs:subClassOf rdf:resource="https://www.wikidata.org/wiki/Q58778"/>
        <rdfs:comment xml:lang="de">Art von System</rdfs:comment>
        <rdfs:comment xml:lang="en">system composed of many interacting components</rdfs:comment>
        <rdfs:comment xml:lang="fr">type de système</rdfs:comment>
        <rdfs:label xml:lang="en">complex system</rdfs:label>
        <rdfs:label xml:lang="de">komplexes System</rdfs:label>
        <rdfs:label xml:lang="fr">système complexe</rdfs:label>
    </owl:Class>
    


    <!-- https://www.wikidata.org/wiki/Q93978369 -->

    <owl:Class rdf:about="https://www.wikidata.org/wiki/Q93978369">
        <rdfs:subClassOf rdf:resource="https://www.wikidata.org/wiki/Q286897"/>
        <rdfs:label xml:lang="de">CBRN-Erkundungswagen</rdfs:label>
    </owl:Class>
    


    <!-- https://www.wikidata.org/wiki/Q99527517 -->

    <owl:Class rdf:about="https://www.wikidata.org/wiki/Q99527517">
        <rdfs:subClassOf rdf:resource="http://purl.obolibrary.org/obo/BFO_0000001"/>
        <rdfs:comment xml:lang="en">entity that is a composite of other entities</rdfs:comment>
        <rdfs:comment xml:lang="fr">entité qui est un composite d&apos;autres entités</rdfs:comment>
        <rdfs:label xml:lang="en">collective entity</rdfs:label>
        <rdfs:label xml:lang="fr">entité composée</rdfs:label>
    </owl:Class>
</rdf:RDF>



<!-- Generated by the OWL API (version 4.5.29.2024-05-13T12:11:03Z) https://github.com/owlcs/owlapi -->

